Source/Dafny/Compilers/Compiler-go.cs
@@ -1004,10 +1004,6 @@ namespace Microsoft.Dafny {
         return Compiler.CreateMethod(m, typeArgs, createBody, ClassName, AbstractMethodWriter, ConcreteMethodWriter, forBodyInheritance, lookasideBody);
       }
 
-      public ConcreteSyntaxTree CreateFreshMethod(Method m) {
-        throw new NotImplementedException();
-      }
-
       public ConcreteSyntaxTree CreateMockMethod(Method m, List<TypeArgumentInstantiation> typeArgs, bool createBody, bool forBodyInheritance, bool lookasideBody) {
         throw new NotImplementedException();
       }
