docs/DafnyRef/Attributes.md
@@ -385,6 +385,39 @@ They are translated into Boogie triggers.
 The `{:typeQuantifier}` attribute must be used on a quantifier if it
 quantifies over types.
 
+### 22.1.21. mock
+
+The `{:mock}` attribute must be used on methods that have no body and return 
+one or more fresh objects. During compilation, if the `/compileMocks` 
+command-line argument is used, the postconditions associated with such a 
+method are translated to a series of API calls to the target languages's 
+mocking framework. The object returned, therefore, behaves exactly as the 
+postconditions specify. If there is a possibility that this behavior violates 
+the specifications on the object's instance methods or hardcodes the values of 
+its fields, the compiler will throw an error but the compilation will go 
+through. Currently, this compilation pass is only supported in C# and requires 
+adding the latest version of the Moq library to the .csproj file before 
+generating the binary.
+
+Not all Dafny postconditions can be translated to calls in Moq - below is the 
+grammar for postconditions that are supported (`S` is the start symbol, `EXPR` 
+stands for an arbitrary Dafny expression, and `ID` stands for 
+variable/method/type identifiers):
+
+```
+S         = FORALL
+          | EQUALS
+          | S && S
+EQUALS    = ID.ID (ARGLIST) == EXPR // stubs a function call
+          | ID.ID           == EXPR // stubs field access
+          | EQUALS && EQUALS
+FORALL    = forall BOUNDVARS :: EXPR ==> EQUALS
+ARGLIST   = ID   // this can be one of the bound variables
+          | EXPR // this expr may not reference any of the bound variables
+          | ARGLIST, ARGLIST
+BOUNDVARS = ID : ID
+          | BOUNDVARS, BOUNDVARS
+```
 
 ## 22.2. Boogie Attributes
 Use the Boogie "/attrHelp" option to get the list of attributes
